ะฃัะฐะฒะฝะตะฝะธะต ะฒะธะดะฐ $ax+by=c$, ะฒ ะบะพัะพัะพะผ $x$, $y$ - ะฝะตะธะทะฒะตััะฝัะต, $aโ0$ ะธะปะธ $bโ0$, ะฐ $c$ - ัะฒะพะฑะพะดะฝัะน ัะปะตะฝ ะฝะฐะทัะฒะฐะตััั ะปะธะฝะตะนะฝัะผะธ ััะฐะฒะฝะตะฝะธัะผะธ ั ะดะฒัะผั ะฝะตะธะทะฒะตััะฝัะผะธ.

>ะฃัะฐะฒะฝะตะฝะธะต ั ะดะฒัะผั ะฝะตะธะทะฒะตััะฝัะผะธ ะธะผะตะตั ะบะฐะบ ะฟัะฐะฒะธะปะพ ะฑะตัะบะพะฝะตัะฝะพ ะผะฝะพะณะพ ัะตัะตะฝะธะน.

**ะะปะณะพัะธัะผ ัะตัะตะฝะธั**
 1. ะััะฐะทะธะผ x ัะตัะตะท y
	$5x+6y=28$
	$6y=-5x+28$
2. ะะฐะดะฐะดะธะผ x=0
	$6y=-5*0+28$
3. ะะตัะธะผ ะฟะพะปััะธะฒัะตะตัั ััะฐะฒะฝะตะฝะธะต
	$6y=28$
	$y=\frac{28}{6} = 4\frac{4}{6} = 4\frac{2}{3}$
4. ะัะฒะตั: (0; $4\frac{2}{3}$)

ะะฒะฐ ััะฐะฒะฝะตะฝะธั, ะธะผะตััะธะต ะพะดะฝะพ ะธ ัะพ ะถะต ะผะฝะพะถะตััะฒะพ ัะตัะตะฝะธะน, ะฝะฐะทัะฒะฐัั ==ัะฐะฒะฝะพัะธะปัะฝัะผะธ ััะฐะฒะฝะตะฝะธัะผะธ==.

ะะพัะบะพะปัะบั $ax+by=c$ ะผะพะถะฝะพ ะฟัะธะฒะตััะธ ะบ ะฒะธะดั $y=-\frac{ax}{b}+\frac{c}{b}$, ัะพ ะณัะฐัะธะบะพะผ ะปะธะฝะตะนะฝะพะณะพ ััะฐะฒะฝะตะฝะธั ั ะดะฒัะผั ะฝะตะธะทะฒะตััะฝัะผะธ ะฟัะธ $bโ0$ ะฑัะดะตั ะฝะตะฒะตััะธะบะฐะปัะฝะฐั ะฟััะผะฐั.

>ะัะปะธ $a=0$; ัะพ $by=c$; ะฟััะผะฐั ะฟะฐัะฐะปะปะตะปัะฝะฐ $ox$
>ะัะปะธ $b=0$; ัะพ ะฟััะผะฐั ะฟะฐัะฐะปะปะตะปัะฝะฐ $oy$
>$0x+0y=0$ - ะัะฐัะธะบ - ะบะพะพัะดะธะฝะฐัะฝะฐั ะฟะปะพัะบะพััั
>$0x+0y=c$ - ะัััะพะต ะผะฝะพะถะตััะฒะพ

---
โฌ๏ธ[[๐ะะธะบะฒะฐะดัะฐัะฝัะต ััะฐะฒะฝะตะฝะธั]]
[[๐ะกะธััะตะผะฐ ััะฐะฒะฝะตะฝะธะน]]โก๏ธ